update examples

Examples.thy
@@ -2,55 +2,143 @@ theory Examples
   imports Earley_List
 begin
 
-subsection \<open>Example 1\<close>
+declare [[names_short]]
 
-datatype t = a | plus
-datatype n = S
-datatype s = Terminal t | Nonterminal n
+subsection \<open>Example 1: Addition\<close>
 
-definition nonterminals :: "s list" where
-  "nonterminals = [Nonterminal S]"
+datatype t1 = x | plus
+datatype n1 = S
+datatype s1 = Terminal t1 | Nonterminal n1
 
-definition terminals :: "s list" where
-  "terminals = [Terminal a, Terminal plus]"
+definition nonterminals1 :: "s1 list" where
+  "nonterminals1 = [Nonterminal S]"
 
-definition rules :: "s rule list" where
-  "rules = [
-    (Nonterminal S, [Terminal a]),
+definition terminals1 :: "s1 list" where
+  "terminals1 = [Terminal x, Terminal plus]"
+
+definition rules1 :: "s1 rule list" where
+  "rules1 = [
+    (Nonterminal S, [Terminal x]),
     (Nonterminal S, [Nonterminal S, Terminal plus, Nonterminal S])
   ]"
 
-definition start_symbol :: s where
-  "start_symbol = Nonterminal S"
+definition start_symbol1 :: s1 where
+  "start_symbol1 = Nonterminal S"
 
-definition cfg :: "s cfg" where
-  "cfg = CFG nonterminals terminals rules start_symbol"
+definition cfg1 :: "s1 cfg" where
+  "cfg1 = CFG nonterminals1 terminals1 rules1 start_symbol1"
 
-definition inp :: "s list" where
-  "inp = [Terminal a, Terminal plus, Terminal a, Terminal plus, Terminal a]"
+definition inp1 :: "s1 list" where
+  "inp1 = [Terminal x, Terminal plus, Terminal x, Terminal plus, Terminal x]"
 
-lemmas cfg_defs = cfg_def nonterminals_def terminals_def rules_def start_symbol_def
+lemmas cfg1_defs = cfg1_def nonterminals1_def terminals1_def rules1_def start_symbol1_def
 
-lemma wf_cfg:
-  "wf_cfg cfg"
-  by (auto simp: wf_cfg_defs cfg_defs)
+lemma wf_cfg1:
+  "wf_cfg cfg1"
+  by (auto simp: wf_cfg_defs cfg1_defs)
 
-lemma is_word_inp:
-  "is_word cfg inp"
-  by (auto simp: is_word_def is_terminal_def cfg_defs inp_def)
+lemma is_word_inp1:
+  "is_word cfg1 inp1"
+  by (auto simp: is_word_def is_terminal_def cfg1_defs inp1_def)
 
-lemma nonempty_derives:
-  "nonempty_derives cfg"
-  by (auto simp: \<epsilon>_free_def cfg_defs rule_body_def nonempty_derives_def \<epsilon>_free_impl_non_empty_deriv)
+lemma nonempty_derives1:
+  "nonempty_derives cfg1"
+  by (auto simp: \<epsilon>_free_def cfg1_defs rule_body_def nonempty_derives_def \<epsilon>_free_impl_non_empty_deriv)
 
-lemma correctness:
-  "earley_recognized_it (\<II>_it cfg inp) cfg inp \<longleftrightarrow> derives cfg [\<SS> cfg] inp"
-  using correctness_list wf_cfg is_word_inp nonempty_derives by blast
+lemma correctness1:
+  "earley_recognized_it (\<II>_it cfg1 inp1) cfg1 inp1 \<longleftrightarrow> derives cfg1 [\<SS> cfg1] inp1"
+  using correctness_list wf_cfg1 is_word_inp1 nonempty_derives1 by blast
 
-value "\<II>_it cfg inp"
-value "earley_recognized_it (\<II>_it cfg inp) cfg inp"
-value "build_dtree cfg inp (\<II>_it cfg inp)"
+value "\<II>_it cfg1 inp1"
+value "earley_recognized_it (\<II>_it cfg1 inp1) cfg1 inp1"
+value "build_tree cfg1 inp1 (\<II>_it cfg1 inp1)"
 
 export_code earley_recognized_it in SML
+
+subsection \<open>Example 2: Addition performance sanity check\<close>
+
+fun size_bins :: "'a bins \<Rightarrow> nat" where
+  "size_bins bs = fold (+) (map length bs) 0"
+
+definition inp1' :: "s1 list" where
+  "inp1' = [
+    Terminal x, Terminal plus, Terminal x, Terminal plus, Terminal x, Terminal plus,
+    Terminal x, Terminal plus, Terminal x, Terminal plus, Terminal x, Terminal plus,
+    Terminal x, Terminal plus, Terminal x, Terminal plus, Terminal x, Terminal plus,
+    Terminal x, Terminal plus, Terminal x, Terminal plus, Terminal x, Terminal plus,
+    Terminal x, Terminal plus, Terminal x, Terminal plus, Terminal x, Terminal plus,
+    Terminal x, Terminal plus, Terminal x, Terminal plus, Terminal x, Terminal plus,
+    Terminal x, Terminal plus, Terminal x, Terminal plus, Terminal x, Terminal plus,
+    Terminal x, Terminal plus, Terminal x, Terminal plus, Terminal x, Terminal plus,
+    Terminal x, Terminal plus, Terminal x, Terminal plus, Terminal x, Terminal plus,
+    Terminal x, Terminal plus, Terminal x, Terminal plus, Terminal x, Terminal plus,
+    Terminal x, Terminal plus, Terminal x, Terminal plus, Terminal x, Terminal plus,
+    Terminal x, Terminal plus, Terminal x, Terminal plus, Terminal x, Terminal plus,
+    Terminal x, Terminal plus, Terminal x, Terminal plus, Terminal x, Terminal plus,
+    Terminal x, Terminal plus, Terminal x, Terminal plus, Terminal x
+  ]"
+
+lemma is_word_inp1':
+  "is_word cfg1 inp1'"
+  by (auto simp: is_word_def is_terminal_def cfg1_defs inp1'_def)
+
+lemma correctness1':
+  "earley_recognized_it (\<II>_it cfg1 inp1') cfg1 inp1' \<longleftrightarrow> derives cfg1 [\<SS> cfg1] inp1'"
+  using correctness_list wf_cfg1 is_word_inp1' nonempty_derives1 by blast
+
+value "\<II>_it cfg1 inp1'"
+value "size_bins (\<II>_it cfg1 inp1')"
+value "earley_recognized_it (\<II>_it cfg1 inp1') cfg1 inp1'"
+value "build_tree cfg1 inp1' (\<II>_it cfg1 inp1')"
+
+subsection \<open>Example 3: Cyclic reduction pointers\<close>
+
+datatype t2 = x
+datatype n2 = A | B
+datatype s2 = Terminal t2 | Nonterminal n2
+
+definition nonterminals2 :: "s2 list" where
+  "nonterminals2 = [Nonterminal A, Nonterminal B]"
+
+definition terminals2 :: "s2 list" where
+  "terminals2 = [Terminal x]"
+
+definition rules2 :: "s2 rule list" where
+  "rules2 = [
+    (Nonterminal A, [Terminal x]),
+    (Nonterminal A, [Nonterminal B]),
+    (Nonterminal B, [Nonterminal A])
+  ]"
+
+definition start_symbol2 :: s2 where
+  "start_symbol2 = Nonterminal A"
+
+definition cfg2 :: "s2 cfg" where
+  "cfg2 = CFG nonterminals2 terminals2 rules2 start_symbol2"
+
+definition inp2 :: "s2 list" where
+  "inp2 = [Terminal x]"
+
+lemmas cfg2_defs = cfg2_def nonterminals2_def terminals2_def rules2_def start_symbol2_def
+
+lemma wf_cfg2:
+  "wf_cfg cfg2"
+  by (auto simp: wf_cfg_defs cfg2_defs)
+
+lemma is_word_inp2:
+  "is_word cfg2 inp2"
+  by (auto simp: is_word_def is_terminal_def cfg2_defs inp2_def)
+
+lemma nonempty_derives2:
+  "nonempty_derives cfg2"
+  by (auto simp: \<epsilon>_free_def cfg2_defs rule_body_def nonempty_derives_def \<epsilon>_free_impl_non_empty_deriv)
+
+lemma correctness2:
+  "earley_recognized_it (\<II>_it cfg2 inp2) cfg2 inp2 \<longleftrightarrow> derives cfg2 [\<SS> cfg2] inp2"
+  using correctness_list wf_cfg2 is_word_inp2 nonempty_derives2 by blast
+
+value "\<II>_it cfg2 inp2"
+value "earley_recognized_it (\<II>_it cfg2 inp2) cfg2 inp2"
+value "build_tree cfg2 inp2 (\<II>_it cfg2 inp2)" \<comment>\<open>TODO: this should not terminate in case of a forest\<close>
 
 end
